update examples

Dafny/examples/simple.i.dfy
@@ -36,177 +36,76 @@ function method{:opaque} lvm_code_Add_single(dst:lvm_operand_opr, size:nat, src1
 
 lemma lvm_lemma_Add_single(lvm_b0:lvm_codes, lvm_s0:lvm_state, lvm_sN:lvm_state, 
             dst:lvm_operand_opr, size:nat, src1:lvm_operand_opr,src2:lvm_operand_opr)
-  returns (lvm_bM:lvm_codes, lvm_sM:lvm_state)
-  requires src1.D?;
+  returns (lvm_bM:lvm_codes, lvm_sM:lvm_state,lvm_sMs:seq<lvm_state>)
   requires lvm_require(lvm_b0, lvm_code_Add_single(dst, size,src1), lvm_s0, lvm_sN)
   requires lvm_is_dst_opr(dst, lvm_s0)
   requires lvm_is_src_opr(src1, lvm_s0)
-  requires lvm_get_ok(lvm_s0)
+  requires ValidState(lvm_s0)
 
   requires ValidOperand(lvm_s0,src1);
   requires OperandContents(lvm_s0,src1).Int?;
-  requires lvm_code_Add_single(dst, size,src1).Ins?;
-  requires ValidOperand(lvm_s0,dst)
+  requires ValidOperand(lvm_s0,src2);
+  requires OperandContents(lvm_s0,src2).Int?;
+  requires ValidOperand(lvm_s0,dst);
+  requires typesMatch(OperandContents(lvm_s0,src1),Int(4,IntType(1,false)));
+  requires size == OperandContents(lvm_s0,src1).itype.size
+  // requires lvm_code_Add(dst, size,src1,src2).Ins?;
 //   
   ensures  lvm_ensure(lvm_b0, lvm_bM, lvm_s0, lvm_sM, lvm_sN)
   ensures  lvm_get_ok(lvm_sM)
   ensures  ValidOperand(lvm_sM,dst)
   ensures  OperandContents(lvm_sM,dst).Int?;
-  ensures  OperandContents(lvm_s0,dst).Int?;
+  ensures  OperandContents(lvm_sM,dst).Int?;
   ensures  OperandContents(lvm_sM, dst).val == 
-  evalADD(OperandContents(lvm_s0,dst).itype.size,OperandContents(lvm_s0,src1),D(Int(4,src1.d.itype)).d).val;
-  ensures  OperandContents(lvm_sM, dst).val == OperandContents(lvm_s0, dst).val + 4
+  evalADD(OperandContents(lvm_s0,src1).itype.size,OperandContents(lvm_s0,src1),D(Int(4,IntType(1,false))).d).val;
+  // ensures  OperandContents(lvm_sM, dst).val == OperandContents(lvm_s0, src1).val + 4
   ensures  lvm_state_eq(lvm_sM, lvm_update_ok(lvm_sM, lvm_update_all( lvm_sM, lvm_s0)))
-  ensures  forall s2 :: evalCode(lvm_b0.hd, lvm_s0, s2) ==> s2.ok
+    ensures lvm_sM.ok ==> ValidStateSeq(lvm_sMs);
 
 {
     reveal_lvm_code_Add_single();
-    assert lvm_code_Add_single(dst, size,src1).Ins?;
-    var addIns := lvm_code_Add_single(dst, size,src1).ins;
-    assert ValidInstruction(lvm_s0,addIns);
-
-    assert  ValidRegOperand(lvm_s0, dst);
-    assert ValidState(lvm_s0);
-    assert lvm_b0.hd.Ins?;
-    var lvm_old_s:lvm_state := lvm_s0;
-    ghost var lvm_ltmp1, lvm_cM:lvm_code, lvm_ltmp2 := lvm_lemma_block(lvm_b0, lvm_s0, lvm_sN);
-    lvm_sM := lvm_ltmp1;
-    lvm_bM := lvm_ltmp2;
-    assert lvm_b0.tl == lvm_bM;
-    assert lvm_bM.CNil?;
-
-    assert evalCode_lax(lvm_cM, lvm_s0, lvm_sM);
-    assert OperandContents(lvm_sM, dst).val == OperandContents(lvm_s0, dst).val + 4;
-
+    reveal_ValidData();
     reveal_evalCodeOpaque();
-}
-
-function method {:opaque} lvm_code_Add_Multiple(dst:lvm_operand_opr, size:nat, src1:lvm_operand_opr): (out:lvm_code)
-    requires src1.D?;
-    requires src1.d.Int?;
-    ensures out.Block?;
-    ensures out.block.lvm_CCons?;
-    ensures out.block.hd.Ins?;
-
-{
-      reveal_IntFits();
-      var val := D(Int(4,src1.d.itype));
-      assert val.d.Int?;
-      var void := D(Void);
-
-      var val2 := D(Int(5,src1.d.itype));
-      assert val.d.Int?;
-
-          lvm_Block(lvm_CCons(Ins(ADD(dst,size,src1,val)),
-                lvm_CCons(Ins(ADD(dst,size,src1,val2)),
-                lvm_CCons(Ins(RET(void)),lvm_CNil()))))
-
-}
-
-lemma lvm_lemma_Add_Multiple(lvm_b0:lvm_codes, lvm_s0:lvm_state, lvm_sN:lvm_state, 
-            dst:lvm_operand_opr, size:nat, src1:lvm_operand_opr,src2:lvm_operand_opr)
-  returns (lvm_bM:lvm_codes, lvm_sM:lvm_state)
-  requires src1.D?;
-  requires src1.d.Int?;
-  requires lvm_require(lvm_b0, lvm_code_Add_Multiple(dst, size,src1), lvm_s0, lvm_sN)
-  requires lvm_is_dst_opr(dst, lvm_s0)
-  requires lvm_is_src_opr(src1, lvm_s0)
-  requires lvm_get_ok(lvm_s0)
-
-  requires ValidOperand(lvm_s0,src1);
-  requires OperandContents(lvm_s0,src1).Int?;
-  requires ValidOperand(lvm_s0,dst);
-  requires ValidOperand(lvm_s0,dst);
-  requires OperandContents(lvm_s0,dst).Int?;
-
-  requires ValidOperand(lvm_s0,dst)
-//   
-  ensures  lvm_ensure(lvm_b0, lvm_bM, lvm_s0, lvm_sM, lvm_sN)
-  ensures  lvm_get_ok(lvm_sM) 
-  ensures ValidOperand(lvm_sM,dst)
-  ensures OperandContents(lvm_sM,dst).Int?;
-  ensures OperandContents(lvm_s0,dst).Int?;
-
-  ensures  OperandContents(lvm_sM, dst).val == evalADD(OperandContents(lvm_s0,dst).itype.size,OperandContents(lvm_s0,src1),D(Int(5,src1.d.itype)).d).val;
-  ensures ToTwosComp(OperandContents(lvm_sM, dst)).val == 
-          (OperandContents(lvm_s0, src1).val + D(Int(5,src1.d.itype)).d.val) % Pow256(OperandContents(lvm_s0, src1).itype.size)
-  ensures  lvm_state_eq(lvm_sM, lvm_update_ok(lvm_sM, lvm_update_all( lvm_sM, lvm_s0)))
-{
-    reveal_lvm_code_Add_Multiple();
     reveal_eval_code();
-    reveal_evalCodeOpaque();
     reveal_lvm_code_Add();
-    reveal_lvm_code_Ret();
-
-    assert lvm_code_Add_Multiple(dst, size,src1).block.hd.Ins?;
-
+    lvm_sMs := [lvm_s0];
+    assert lvm_code_Add_single(dst,size,src1).block.hd.Ins?;
     assert ValidState(lvm_s0);
-    var lvm_old_s:lvm_state := lvm_s0;
-    assert evalCode(lvm_Block(lvm_b0), lvm_s0, lvm_sN);
-    assert eval_code(lvm_Block(lvm_b0), lvm_s0, lvm_sN);
+    assert lvm_code_Add_single(dst, size,src1).block.hd.ins == ADD(dst, size,src1,D(Int(4,IntType(1,false))));
+    assert ValidInstruction(lvm_s0,lvm_code_Add_single(dst,size,src1).block.hd.ins);
+    assert lvm_b0.hd.Block?;
+    assert lvm_b0.hd.block.hd.ins == ADD(dst, size,src1,D(Int(4,IntType(1,false))));
+    assert lvm_b0.hd.block == lvm_code_Add_single(dst,size,src1).block;
+
+    assert evalBlock(lvm_b0,lvm_s0, lvm_sN);
+    // assert  ValidRegOperand(lvm_s0, dst);
 
     ghost var lvm_ltmp1, lvm_cM:lvm_code, lvm_ltmp2 := lvm_lemma_block(lvm_b0, lvm_s0, lvm_sN);
     lvm_sM := lvm_ltmp1;
     lvm_bM := lvm_ltmp2;
     var lvm_b1:lvm_codes := lvm_get_block(lvm_cM);
-    assert lvm_b1.lvm_CCons?;
-    reveal_IntFits();
-    var val := D(Int(4,src1.d.itype));
-    assert val.d.Int?;
-    assert lvm_b1.hd == lvm_code_Add(dst, size,src1,val);
-    assert ValidState(lvm_s0);
-    assert evalCode_lax(lvm_Block(lvm_b1), lvm_s0, lvm_sM);
-    assert OperandContents(lvm_s0,dst).Int?;
-
-    // assert evalUpdate(lvm_s0, dst, evalADD(size,OperandContents(lvm_s0,src1),OperandContents(lvm_s0,val)),lvm_sM);
-    assert evalCode(lvm_Block(lvm_b1), lvm_s0, lvm_sM);
-    assert evalBlock(lvm_Block(lvm_b1).block, lvm_s0, lvm_sM);
-    assert lvm_Block(lvm_b1).block.hd == Ins(ADD(dst, size,src1,val));
-    assert  exists r' ::  evalCode(lvm_b1.hd, lvm_s0, r');
-    assert  exists r' ::  evalIns(lvm_b1.hd.ins, lvm_s0, r');
-
-    var val2 := D(Int(5,src1.d.itype));
-    var step1 := evalADD(OperandContents(lvm_s0,dst).itype.size,OperandContents(lvm_s0,src1),val.d);
+    assert lvm_b0.tl == lvm_bM;
+    ghost var lvm_b2, lvm_s2 := lvm_lemma_Add(lvm_b1, lvm_s0, lvm_sM, dst, size,src1,D(Int(4,IntType(1,false))));
+    assert StateNext(lvm_s0,lvm_s2);
+    lvm_sMs := lvm_sMs + [lvm_s2];
 
 
-    ghost var lvm_b2, lvm_s2 := lvm_lemma_Add(lvm_b1, lvm_s0, lvm_sM, dst, size,src1,val);
+    assert lvm_b2 == (lvm_CNil());
+    assert eval_code(lvm_Block(lvm_b2), lvm_s2, lvm_sM);
+    lvm_sM := lvm_lemma_empty(lvm_s2,lvm_sM);
+    assert ValidState(lvm_sM);
+    assert StateNext(lvm_s2,lvm_sM);
+    lvm_sMs := lvm_sMs + [lvm_sM];
 
-
-    assert OperandContents(lvm_s2, dst).val == step1.val;
-    assert OperandContents(lvm_s0, src1) == OperandContents(lvm_s2, src1); 
-
-    assert  lvm_require(lvm_b2, lvm_code_Add(dst, size,src1,val2), lvm_s2, lvm_sM);
-    var step2 := evalADD(OperandContents(lvm_s2,dst).itype.size,OperandContents(lvm_s2,src1),val2.d);
-
-    ghost var lvm_b3, lvm_s3 := lvm_lemma_Add(lvm_b2, lvm_s2, lvm_sM, dst, size,src1,val2);
-    assert OperandContents(lvm_s3, dst).val 
-        == evalADD(OperandContents(lvm_s2,dst).itype.size,OperandContents(lvm_s2,src1),val2.d).val;
-  
-    assert OperandContents(lvm_s3, dst).val  == step2.val;
-    // assert lvm_b3.CNil?;
-    assert lvm_b3.hd.ins == RET(D(Void));
-
-    
-    ghost var lvm_b4, lvm_s4 := lvm_lemma_Ret(lvm_b3, lvm_s3, lvm_sM, dst, D(Void));
-    assert lvm_b4.CNil?;
-    assert eval_code(lvm_Block(lvm_b4), lvm_s4, lvm_sM);
-    lvm_sM := lvm_lemma_empty(lvm_s4,lvm_sM);
-    assert   OperandContents(lvm_sM, dst).val  == step2.val;
 
     assert evalCode_lax(lvm_cM, lvm_s0, lvm_sM);
-    assert OperandContents(lvm_s0, src1) == OperandContents(lvm_sM, src1); 
-
-    assert OperandContents(lvm_sM, dst).val == step2.val;
-    assert  OperandContents(lvm_sM, dst).val == evalADD(OperandContents(lvm_s0,dst).itype.size,OperandContents(lvm_s0,src1),val2.d).val;
-    assert ValidState(lvm_sM);
     reveal_evalCodeOpaque();
 }
 
 
-
 // ////
 
-function method {:opaque} lvm_code_Add_Multiple1(dst:lvm_operand_opr, size:nat, src1:lvm_operand_opr, src2:lvm_operand_opr): (out:lvm_code)
+function method {:opaque} lvm_code_Add_Multiple(dst:lvm_operand_opr, size:nat, src1:lvm_operand_opr, src2:lvm_operand_opr): (out:lvm_code)
     requires src1.D?;
     requires src1.d.Int?;
     requires src2.D?;
@@ -224,22 +123,20 @@ function method {:opaque} lvm_code_Add_Multiple1(dst:lvm_operand_opr, size:nat, 
       var val2 := D(Int(5,src2.d.itype));
       assert val.d.Int?;
 
-      // var void := D(Void);
-
       lvm_Block(lvm_CCons(Ins(ADD(src2,size,src1,val)),
                 lvm_CCons(Ins(ADD(dst,size,src2,val2)),
                 lvm_CCons(Ins(RET(void)),lvm_CNil()))))
 
 }
 
-lemma lvm_lemma_Add_Multiple1(lvm_b0:lvm_codes, lvm_s0:lvm_state, lvm_sN:lvm_state, 
+lemma lvm_lemma_Add_Multiple(lvm_b0:lvm_codes, lvm_s0:lvm_state, lvm_sN:lvm_state, 
             dst:lvm_operand_opr, size:nat, src1:lvm_operand_opr,src2:lvm_operand_opr)
-  returns (lvm_bM:lvm_codes, lvm_sM:lvm_state)
+  returns (lvm_bM:lvm_codes, lvm_sM:lvm_state,lvm_sMs:seq<lvm_state>)
   requires src1.D?;
   requires src1.d.Int?;
   requires src2.D?;
   requires src2.d.Int?;
-  requires lvm_require(lvm_b0, lvm_code_Add_Multiple1(dst, size,src1,src2), lvm_s0, lvm_sN)
+  requires lvm_require(lvm_b0, lvm_code_Add_Multiple(dst, size,src1,src2), lvm_s0, lvm_sN)
   requires lvm_is_dst_opr(dst, lvm_s0)
   requires lvm_is_dst_opr(src2, lvm_s0)
   requires lvm_is_src_opr(src1, lvm_s0)
@@ -250,26 +147,31 @@ lemma lvm_lemma_Add_Multiple1(lvm_b0:lvm_codes, lvm_s0:lvm_state, lvm_sN:lvm_sta
   requires ValidOperand(lvm_s0,src2);
   requires OperandContents(lvm_s0,src2).Int?;
   requires ValidOperand(lvm_s0,dst);
-  requires OperandContents(lvm_s0,dst).Int?;
+  requires typesMatch(OperandContents(lvm_s0,src1),Int(4,src1.d.itype));
+    requires typesMatch(OperandContents(lvm_s0,src2),Int(5,src2.d.itype));
+
+  requires size == OperandContents(lvm_s0,src1).itype.size && size == OperandContents(lvm_s0,src2).itype.size 
 //   
   ensures  lvm_ensure(lvm_b0, lvm_bM, lvm_s0, lvm_sM, lvm_sN)
   ensures  lvm_get_ok(lvm_sM) 
   ensures ValidOperand(lvm_sM,dst)
   ensures OperandContents(lvm_sM,dst).Int?;
-  ensures OperandContents(lvm_s0,dst).Int?;
 
-  ensures OperandContents(lvm_sM, dst).val == evalADD(OperandContents(lvm_s0,dst).itype.size,OperandContents(lvm_s0,src2),D(Int(5,src2.d.itype)).d).val
+  ensures OperandContents(lvm_sM, dst).val == evalADD(OperandContents(lvm_s0,src1).itype.size,OperandContents(lvm_s0,src2),D(Int(5,src2.d.itype)).d).val
   // ensures ToTwosComp(OperandContents(lvm_sM, dst)).val == 
           // (OperandContents(lvm_s0, src1).val + D(Int(5,src1.d.itype)).d.val + D(Int(4,src1.d.itype)).d.val ) % Pow256(OperandContents(lvm_s0, src1).itype.size)
   ensures  lvm_state_eq(lvm_sM, lvm_update_ok(lvm_sM, lvm_update_all( lvm_sM, lvm_s0)))
+  ensures lvm_sM.ok ==> ValidStateSeq(lvm_sMs);
+
 {
-    reveal_lvm_code_Add_Multiple1();
+    reveal_lvm_code_Add_Multiple();
     reveal_eval_code();
     reveal_evalCodeOpaque();
     reveal_lvm_code_Add();
-      reveal_lvm_code_Ret();
+    reveal_lvm_code_Ret();
+    lvm_sMs := [lvm_s0];
 
-    assert lvm_code_Add_Multiple1(dst, size,src1,src2).block.hd.Ins?;
+    assert lvm_code_Add_Multiple(dst, size,src1,src2).block.hd.Ins?;
 
     assert ValidState(lvm_s0);
     var lvm_old_s:lvm_state := lvm_s0;
@@ -307,11 +209,10 @@ lemma lvm_lemma_Add_Multiple1(lvm_b0:lvm_codes, lvm_s0:lvm_state, lvm_sN:lvm_sta
 
     var val2 := D(Int(5,src2.d.itype));
     var step1 := evalADD(OperandContents(lvm_s0,src2).itype.size,OperandContents(lvm_s0,src1),val.d);
-        assert OperandContents(lvm_s0,dst).Int?;
-
 
     ghost var lvm_b2, lvm_s2 := lvm_lemma_Add(lvm_b1, lvm_s0, lvm_sM, src2, size,src1,val);
-
+    assert StateNext(lvm_s0,lvm_s2);
+    lvm_sMs := lvm_sMs + [lvm_s2];
 
     assert OperandContents(lvm_s2, src2).val == step1.val;
     assert OperandContents(lvm_s2,src2).val == evalADD(size,OperandContents(lvm_s0,src1),OperandContents(lvm_s0,val)).val;
@@ -323,8 +224,10 @@ lemma lvm_lemma_Add_Multiple1(lvm_b0:lvm_codes, lvm_s0:lvm_state, lvm_sN:lvm_sta
     // var step2 := evalADD(OperandContents(lvm_s2,dst).itype.size,OperandContents(lvm_s2,src2),val2.d);
 
     ghost var lvm_b3, lvm_s3 := lvm_lemma_Add(lvm_b2, lvm_s2, lvm_sM, dst, size,src2,val2);
+    assert StateNext(lvm_s2,lvm_s3);
+    lvm_sMs := lvm_sMs + [lvm_s3];
     assert OperandContents(lvm_s3, dst).val 
-        == evalADD(OperandContents(lvm_s2,dst).itype.size,OperandContents(lvm_s2,src2),val2.d).val;
+        == evalADD(OperandContents(lvm_s2,src2).itype.size,OperandContents(lvm_s2,src2),val2.d).val;
   
     // assert OperandContents(lvm_s3, dst).val  == step2.val;
 
@@ -332,21 +235,143 @@ lemma lvm_lemma_Add_Multiple1(lvm_b0:lvm_codes, lvm_s0:lvm_state, lvm_sN:lvm_sta
 
     
     ghost var lvm_b4, lvm_s4 := lvm_lemma_Ret(lvm_b3, lvm_s3, lvm_sM, dst, D(Void));
+    assert StateNext(lvm_s3,lvm_s4);
+    lvm_sMs := lvm_sMs + [lvm_s4];
     assert lvm_b4.CNil?;
 
     lvm_sM := lvm_lemma_empty(lvm_s4,lvm_sM);
+    assert StateNext(lvm_s4,lvm_sM);
+    lvm_sMs := lvm_sMs + [lvm_sM];
     // assert OperandContents(lvm_sM, dst).val  == step2.val;
     assert  OperandContents(lvm_s4, dst).val 
-        == evalADD(OperandContents(lvm_s2,dst).itype.size,OperandContents(lvm_s2,src2),val2.d).val;
+        == evalADD(OperandContents(lvm_s2,src2).itype.size,OperandContents(lvm_s2,src2),val2.d).val;
     assert evalCode_lax(lvm_cM, lvm_s0, lvm_sM);
     assert OperandContents(lvm_s0, src1) == OperandContents(lvm_sM, src1); 
-
-    // assert OperandContents(lvm_sM, dst).val == step2.val;
-    assert  OperandContents(lvm_sM, dst).val == evalADD(OperandContents(lvm_s0,dst).itype.size,OperandContents(lvm_s0,src2),val2.d).val;
+    assert  OperandContents(lvm_sM, dst).val == evalADD(OperandContents(lvm_s0,src1).itype.size,OperandContents(lvm_s0,src2),val2.d).val;
     assert ValidState(lvm_sM);
 
     reveal_evalCodeOpaque();
 }
+// Old example // 
+
+// function method {:opaque} lvm_code_Add_Multiple(dst:lvm_operand_opr, size:nat, src1:lvm_operand_opr): (out:lvm_code)
+//     requires src1.D?;
+//     requires src1.d.Int?;
+//     ensures out.Block?;
+//     ensures out.block.lvm_CCons?;
+//     ensures out.block.hd.Ins?;
+
+// {
+//       reveal_IntFits();
+//       var val := D(Int(4,src1.d.itype));
+//       assert val.d.Int?;
+//       var void := D(Void);
+
+//       var val2 := D(Int(5,src1.d.itype));
+//       assert val.d.Int?;
+
+//           lvm_Block(lvm_CCons(Ins(ADD(dst,size,src1,val)),
+//                 lvm_CCons(Ins(ADD(dst,size,src1,val2)),
+//                 lvm_CCons(Ins(RET(void)),lvm_CNil()))))
+
+// }
+
+// lemma lvm_lemma_Add_Multiple(lvm_b0:lvm_codes, lvm_s0:lvm_state, lvm_sN:lvm_state, 
+//             dst:lvm_operand_opr, size:nat, src1:lvm_operand_opr,src2:lvm_operand_opr)
+//   returns (lvm_bM:lvm_codes, lvm_sM:lvm_state)
+//   requires src1.D?;
+//   requires src1.d.Int?;
+//   requires lvm_require(lvm_b0, lvm_code_Add_Multiple(dst, size,src1), lvm_s0, lvm_sN)
+//   requires lvm_is_dst_opr(dst, lvm_s0)
+//   requires lvm_is_src_opr(src1, lvm_s0)
+//   requires lvm_get_ok(lvm_s0)
+
+//   requires ValidOperand(lvm_s0,src1);
+//   requires OperandContents(lvm_s0,src1).Int?;
+//   requires ValidOperand(lvm_s0,dst);
+//   requires ValidOperand(lvm_s0,dst);
+//   requires OperandContents(lvm_s0,dst).Int?;
+
+//   requires ValidOperand(lvm_s0,dst)
+// //   
+//   ensures  lvm_ensure(lvm_b0, lvm_bM, lvm_s0, lvm_sM, lvm_sN)
+//   ensures  lvm_get_ok(lvm_sM) 
+//   ensures ValidOperand(lvm_sM,dst)
+//   ensures OperandContents(lvm_sM,dst).Int?;
+//   ensures OperandContents(lvm_s0,dst).Int?;
+
+//   ensures  OperandContents(lvm_sM, dst).val == evalADD(OperandContents(lvm_s0,dst).itype.size,OperandContents(lvm_s0,src1),D(Int(5,src1.d.itype)).d).val;
+//   ensures ToTwosComp(OperandContents(lvm_sM, dst)).val == 
+//           (OperandContents(lvm_s0, src1).val + D(Int(5,src1.d.itype)).d.val) % Pow256(OperandContents(lvm_s0, src1).itype.size)
+//   ensures  lvm_state_eq(lvm_sM, lvm_update_ok(lvm_sM, lvm_update_all( lvm_sM, lvm_s0)))
+// {
+//     reveal_lvm_code_Add_Multiple();
+//     reveal_eval_code();
+//     reveal_evalCodeOpaque();
+//     reveal_lvm_code_Add();
+//     reveal_lvm_code_Ret();
+
+//     assert lvm_code_Add_Multiple(dst, size,src1).block.hd.Ins?;
+
+//     assert ValidState(lvm_s0);
+//     var lvm_old_s:lvm_state := lvm_s0;
+//     assert evalCode(lvm_Block(lvm_b0), lvm_s0, lvm_sN);
+//     assert eval_code(lvm_Block(lvm_b0), lvm_s0, lvm_sN);
+
+//     ghost var lvm_ltmp1, lvm_cM:lvm_code, lvm_ltmp2 := lvm_lemma_block(lvm_b0, lvm_s0, lvm_sN);
+//     lvm_sM := lvm_ltmp1;
+//     lvm_bM := lvm_ltmp2;
+//     var lvm_b1:lvm_codes := lvm_get_block(lvm_cM);
+//     assert lvm_b1.lvm_CCons?;
+//     reveal_IntFits();
+//     var val := D(Int(4,src1.d.itype));
+//     assert val.d.Int?;
+//     assert lvm_b1.hd == lvm_code_Add(dst, size,src1,val);
+//     assert ValidState(lvm_s0);
+//     assert evalCode_lax(lvm_Block(lvm_b1), lvm_s0, lvm_sM);
+//     assert OperandContents(lvm_s0,dst).Int?;
+
+//     // assert evalUpdate(lvm_s0, dst, evalADD(size,OperandContents(lvm_s0,src1),OperandContents(lvm_s0,val)),lvm_sM);
+//     assert evalCode(lvm_Block(lvm_b1), lvm_s0, lvm_sM);
+//     assert evalBlock(lvm_Block(lvm_b1).block, lvm_s0, lvm_sM);
+//     assert lvm_Block(lvm_b1).block.hd == Ins(ADD(dst, size,src1,val));
+//     assert  exists r' ::  evalCode(lvm_b1.hd, lvm_s0, r');
+//     assert  exists r' ::  evalIns(lvm_b1.hd.ins, lvm_s0, r');
+
+//     var val2 := D(Int(5,src1.d.itype));
+//     var step1 := evalADD(OperandContents(lvm_s0,dst).itype.size,OperandContents(lvm_s0,src1),val.d);
 
 
+//     ghost var lvm_b2, lvm_s2 := lvm_lemma_Add(lvm_b1, lvm_s0, lvm_sM, dst, size,src1,val);
+
+
+//     assert OperandContents(lvm_s2, dst).val == step1.val;
+//     assert OperandContents(lvm_s0, src1) == OperandContents(lvm_s2, src1); 
+
+//     assert  lvm_require(lvm_b2, lvm_code_Add(dst, size,src1,val2), lvm_s2, lvm_sM);
+//     var step2 := evalADD(OperandContents(lvm_s2,dst).itype.size,OperandContents(lvm_s2,src1),val2.d);
+
+//     ghost var lvm_b3, lvm_s3 := lvm_lemma_Add(lvm_b2, lvm_s2, lvm_sM, dst, size,src1,val2);
+//     assert OperandContents(lvm_s3, dst).val 
+//         == evalADD(OperandContents(lvm_s2,dst).itype.size,OperandContents(lvm_s2,src1),val2.d).val;
+  
+//     assert OperandContents(lvm_s3, dst).val  == step2.val;
+//     // assert lvm_b3.CNil?;
+//     assert lvm_b3.hd.ins == RET(D(Void));
+
+    
+//     ghost var lvm_b4, lvm_s4 := lvm_lemma_Ret(lvm_b3, lvm_s3, lvm_sM, dst, D(Void));
+//     assert lvm_b4.CNil?;
+//     assert eval_code(lvm_Block(lvm_b4), lvm_s4, lvm_sM);
+//     lvm_sM := lvm_lemma_empty(lvm_s4,lvm_sM);
+//     assert   OperandContents(lvm_sM, dst).val  == step2.val;
+
+//     assert evalCode_lax(lvm_cM, lvm_s0, lvm_sM);
+//     assert OperandContents(lvm_s0, src1) == OperandContents(lvm_sM, src1); 
+
+//     assert OperandContents(lvm_sM, dst).val == step2.val;
+//     assert  OperandContents(lvm_sM, dst).val == evalADD(OperandContents(lvm_s0,dst).itype.size,OperandContents(lvm_s0,src1),val2.d).val;
+//     assert ValidState(lvm_sM);
+//     reveal_evalCodeOpaque();
+// }
 }
