Dafny/control_flow.i.dfy
@@ -186,21 +186,21 @@ lemma lvm_lemma_block(b:codes, s0:lvm_state, r:lvm_state)
     ensures  eval_code(c0, s0, r1)
     ensures  eval_code(Block(b1), r1, r)
     ensures s0.ok ==> evalCode(b.hd, s0, r1) && evalBlock(b.tl, r1, r);
-    ensures s0.ok && b.hd.Block? ==> r1 == s0;
+    // ensures s0.ok && b.hd.Block? ==> r1 == s0;
 {
     reveal_eval_code();
     c0 := b.hd;
     b1 := b.tl;
     if s0.ok {
         assert evalBlock(b, s0, r);
-        var r':state :| evalCode(b.hd, s0, r') && evalBlock(b.tl, r', r)  && (b.hd.Block? ==> s0 == r');
+        var r':state :| evalCode(b.hd, s0, r') && evalBlock(b.tl, r', r) ;
         r1 := r';
         if ValidState(s0) {
             code_state_validity(c0, s0, r1);
         }
-        if(b.hd.Block?){
-            assert r1 == s0;
-        }
+        // if(b.hd.Block?){
+        //     assert r1 == s0;
+        // }
         assert eval_code(c0, s0, r1);
     } else {
         r1 := s0;
